
### VIMMP CODELISTS (VCL) FOR ZONTAL ###

### VERSION 0.3.0 ###

### DATED 28TH SEPTEMBER 2020 ###

@prefix vcl: <https://purl.vimmp.eu/semantics/alignment/vcl.ttl#>.

@prefix dcterms: <http://purl.org/dc/terms/>.
@prefix evmpo: <https://emmc.eu/semantics/evmpo/evmpo.ttl#>.
@prefix otras: <https://purl.vimmp.eu/semantics/otras/otras.ttl#>.
@prefix owl: <http://www.w3.org/2002/07/owl#>.
@prefix owl2: <http://www.w3.org/2006/12/owl2#>.
@prefix rdf: <http://www.w3.org/1999/02/22-rdf-syntax-ns#>.
@prefix rdfs: <http://www.w3.org/2000/01/rdf-schema#>.
@prefix skos: <http://www.w3.org/2004/02/skos/core#>.
@prefix vico: <https://purl.vimmp.eu/semantics/vico/vico.ttl#>.
@prefix viprs: <https://purl.vimmp.eu/semantics/alignment/viprs.ttl#>.
@prefix xs: <http://www.w3.org/2001/XMLSchema#>.

<https://purl.vimmp.eu/semantics/alignment/vcl.ttl> a owl:Ontology;
   dcterms:title "VCL: VIMMP Codelists"^^xs:string;
   owl:versionInfo "version 0.2.3"^^xs:string;
   dcterms:modified "2020-06-27"^^xs:date;
   dcterms:publisher "Virtual Materials Marketplace (VIMMP) project consortium"^^xs:string;
   dcterms:license "GNU Lesser General Public License (LGPL) version 3"^^xs:string;
   dcterms:creator "Martin Thomas Horsch (ORCID 0000-0002-9464-6739)"^^xs:string;
   dcterms:creator "Silvia Chiacchiera (ORCID 0000-0003-0422-7870)"^^xs:string;
   dcterms:creator "Michael A. Seaton (ORCID 0000-0002-4708-573X)"^^xs:string;
   dcterms:creator "Ilian T. Todorov (ORCID 0000-0001-7275-1784)"^^xs:string;
   dcterms:contributor "Welchy Leite Cavalcanti"^^xs:string;
   dcterms:contributor "Andreas Fiseni"^^xs:string.

vcl:codelist_mm_topic a owl:Class;
   rdfs:subClassOf evmpo:marketplace_related_entity, viprs:conceptualization;
   owl:equivalentClass otras:mm_topic, [
      a owl:Restriction;
      owl:onProperty skos:inScheme;
      owl:hasValue vcl:CL_SCHEME_MM_TOPIC
   ];
   rdfs:comment "materials modelling topic"^^xs:string.
vcl:CL_SCHEME_MM_TOPIC a owl:NamedIndividual, skos:ConceptScheme;
   skos:prefLabel "mm_topic"^^xs:string;
   skos:definition "materials modelling topic"^^xs:string.

vcl:codelist_interlocutor_group a owl:Class;
   rdfs:subClassOf evmpo:annotation, viprs:conceptualization;
   owl:equivalentClass vico:interlocutor_group, [
      a owl:Restriction;
      owl:onProperty skos:inScheme;
      owl:hasValue vcl:CL_SCHEME_INTERLOCUTOR_GROUP
   ];
   rdfs:comment "interlocutor group"^^xs:string.
vcl:CL_SCHEME_INTERLOCUTOR_GROUP a owl:NamedIndividual, skos:ConceptScheme;
   skos:prefLabel "interlocutor_group"^^xs:string;
   skos:definition "interlocutor group"^^xs:string.

###
# DATATYPE PROPERTIES
###

skos:definition a owl:DatatypeProperty;
   rdfs:subPropertyOf viprs:has_descriptor.
skos:prefLabel a owl:DatatypeProperty;
   rdfs:subPropertyOf viprs:has_label.
skos:inScheme a owl:ObjectProperty;
   rdfs:subPropertyOf viprs:is_proper_part_of.
