
### VIMMP PRIMITIVES (VIPRS) ###

### VERSION 0.1.1 ###

### DATED 15TH MAY 2020 ###

# 1. Modal square of opposition
#
# a) individual relations
# b) conceptual relations
#
# 2. Below, categories of primitive properties for EMMO-based mereology and semiotics
#
# a) occurrence and requirement (implied co-occurrence) in the same scenario, possible world, environment, or realization 
#    -> necessity/possibility
#    -> positive/negative
#    -> active/passive
#    -> individual/conceptual
#
# b) proper parthood (eight varieties) - below coexistence
#    -> necessity/possibility
#    -> positive/negative
#    -> active/passive
#
# c) representation (eight varieties) - coexistence not explicitly implied (however, it is indirectly implied through the EMMO)
#    -> necessity/possibility
#    -> positive/negative
#    -> active/passive
#
# 3. Additionally, non-primitives
#
# a) more specific high-level properties
# b) chain properties: mereosemiotics

@prefix viprs: <http://www.vimmp.eu/semantics/alignment/viprs.ttl#>.

@prefix owl: <http://www.w3.org/2002/07/owl#>.
@prefix owl2: <http://www.w3.org/2006/12/owl2#>.
@prefix rdf: <http://www.w3.org/1999/02/22-rdf-syntax-ns#>.
@prefix rdfs: <http://www.w3.org/2000/01/rdf-schema#>.
@prefix xs: <http://www.w3.org/2001/XMLSchema#>.

<http://www.vimmp.eu/semantics/alignment/viprs.ttl> a owl:Ontology.

viprs:meta_emmo a owl:Class;
   rdfs:subClassOf owl:Thing.
viprs:realization a owl:Class;
   rdfs:subClassOf viprs:meta_emmo;
   owl:disjointWith viprs:entity;
   rdfs:comment "realization, i.e., a scenario, possible world, or environment"^^xs:string.
viprs:entity a owl:Class;
   rdfs:subClassOf viprs:meta_emmo;
   owl:disjointWith viprs:realization;
   rdfs:comment "entity, i.e., something that may or may not occur within a realization"^^xs:string.
viprs:occurs_in a owl:ObjectProperty;
   rdfs:domain viprs:entity;
   rdfs:range viprs:realization;
   owl:propertyDisjointWith viprs:does_not_occur_in.
viprs:does_not_occur_in a owl:ObjectProperty;
   rdfs:domain viprs:entity;
   rdfs:range viprs:realization;
   owl:propertyDisjointWith viprs:occurs_in.
viprs:top_relation a owl:ObjectProperty;
   rdfs:domain viprs:entity;
   rdfs:range viprs:entity.

#################################
# 1. MODAL SQUARE OF OPPOSITION #
#################################

# note; for classification purposes, the top relations
# are provided in two versions: individual and conceptual

## 1A. INDIVIDUAL RELATIONS: X relates to Y (below "X P Y", for some P) ##

viprs:individual_necessity a owl:ObjectProperty;
   rdfs:domain viprs:entity;
   rdfs:range viprs:entity;
   rdfs:subPropertyOf viprs:individual_possibility, viprs:conceptual_necessity;
   rdfs:comment "X individual_necessity Y == for some P, in all realizations X P Y"^^xs:string.
viprs:individual_possibility a owl:ObjectProperty;
   rdfs:domain viprs:entity;
   rdfs:range viprs:entity;
   rdfs:subPropertyOf viprs:top_relation;
   rdfs:comment "X individual_possibility Y == for some P, in some realization X P Y"^^xs:string.

## 1B. CONCEPTUAL RELATIONS: X and Y are selected from sets/classes A and B, respectively ##

viprs:conceptual_necessity a owl:ObjectProperty;
   rdfs:domain viprs:entity;
   rdfs:range viprs:entity;
   rdfs:subPropertyOf viprs:top_relation;
   rdfs:comment "X conceptual_necessity Y == for some property P, A concept for X, B concept for Y, in all realizations [some A] P [some B]"^^xs:string.
viprs:conceptual_possibility a owl:ObjectProperty;
   rdfs:domain viprs:entity;
   rdfs:range viprs:entity;
   rdfs:subPropertyOf viprs:individual_possibility;
   rdfs:comment "X conceptual_possibility Y == for some property P, A concept for X, B concept for Y, in some realization [all A] P [all B]"^^xs:string.

############################################
# 2A. OCCURRENCE AND IMPLIED CO-OCCURRENCE #
############################################

# square of opposition for individuals
#
viprs:necessary_entity a owl:Class;
   rdfs:subClassOf viprs:possible_entity;
   owl:equivalentClass [
      owl:intersectionOf (
         viprs:entity [
            a owl:Restriction;
            owl:onProperty viprs:does_not_occur_in;
            owl:cardinality 0
         ]
      )
   ];
   rdfs:comment "necessary entity, i.e., an entity that occurs in every realization"^^xs:string.
viprs:possible_entity a owl:Class;
   rdfs:subClassOf viprs:entity;
   owl:equivalentClass [
      owl:intersectionOf (
         viprs:entity [
            a owl:Restriction;
            owl:onProperty viprs:occurs_in;
            owl:someValuesFrom viprs:realization
         ]
      )
   ];
   rdfs:comment "possible entity, i.e., an entity that occurs in at least one realization"^^xs:string.
viprs:non_necessary_entity a owl:Class;
   rdfs:subClassOf viprs:entity;
   owl:equivalentClass [
      owl:intersectionOf (
         viprs:entity [
            a owl:Restriction;
            owl:onProperty viprs:does_not_occur_in;
            owl:someValuesFrom viprs:realization
         ]
      )
   ];
   rdfs:comment "non-necessary entity, i.e., an entity that does not occur in all realizations"^^xs:string.
viprs:impossible_entity a owl:Class;
   rdfs:subClassOf viprs:non_necessary_entity;
   owl:equivalentClass [
      owl:intersectionOf (
         viprs:entity [
            a owl:Restriction;
            owl:onProperty viprs:occurs_in;
            owl:cardinality 0
         ]
      )
   ];
   rdfs:comment "impossible entity, i.e., an entity that does not occur in any realization"^^xs:string.

viprs:entity owl:disjointUnionOf (viprs:necessary_entity viprs:non_necessary_entity).
viprs:entity owl:disjointUnionOf (viprs:possible_entity viprs:impossible_entity).

# necessary-positive, active, individual
#
viprs:requires a owl:ObjectProperty, owl:TransitiveProperty;
   rdfs:domain viprs:entity;
   rdfs:range viprs:entity;
   rdfs:subPropertyOf viprs:individual_necessity;
   rdfs:comment "X requires Y == in all realizations, Y occurs or X does not occur (i.e., X -> Y)"^^xs:string.

# necessary-positive, passive, individual
#
viprs:is_required_by a owl:ObjectProperty, owl:TransitiveProperty;
   rdfs:domain viprs:entity;
   rdfs:range viprs:entity;
   rdfs:subPropertyOf viprs:individual_necessity;
   rdfs:comment "X is_required_by Y == in all realizations, X occurs or Y does not occur (i.e., Y -> X)"^^xs:string.

# possible-negative, active, individual
#
viprs:does_not_require a owl:ObjectProperty;
   rdfs:domain viprs:possible_entity;
   rdfs:range viprs:non_necessary_entity;
   rdfs:subPropertyOf viprs:individual_possibility;
   rdfs:comment "X does_not_require Y == in some realization, X occurs and Y does not occur (i.e., ![X -> Y])"^^xs:string.

# possible-negative, passive, individual
#
viprs:is_not_required_by a owl:ObjectProperty;
   rdfs:domain viprs:possible_entity;
   rdfs:range viprs:non_necessary_entity;
   rdfs:subPropertyOf viprs:individual_possibility;
   rdfs:comment "X is_not_required_by Y == in some realization, Y occurs and X does not occur (i.e., ![Y -> X])"^^xs:string.

#######################
# 2B. PROPER PARTHOOD #
#######################

######################
# 2C. REPRESENTATION #
######################

###########################################
# 3A. MORE SPECIFIC HIGH-LEVEL PROPERTIES #
###########################################

#####################################
# 3B. MEREOSEMIOTIC CHAIN RELATIONS #
#####################################
